well-formed recursion in the interpreter (expr only)

Interpret.v
@@ -19,25 +19,29 @@ Inductive stmt_abort (return_type: Type)
  | AbortReturnFromContract
  | AbortRevert.
 
-Inductive stmt_result {C: VyperConfig} (return_type: Type)
+Section Interpret.
+
+Context {C: VyperConfig}.
+
+Inductive stmt_result (return_type: Type)
 := StmtSuccess
  | StmtAbort (a: stmt_abort return_type).
-Arguments StmtSuccess {_ _}.
-Arguments StmtAbort {_ _}.
+Arguments StmtSuccess {_}.
+Arguments StmtAbort {_}.
 
 (** XXX *)
-Definition interpret_unop {C: VyperConfig} (op: unop) (a: uint256)
+Definition interpret_unop (op: unop) (a: uint256)
 : expr_result uint256
 := ExprSuccess a.
 
 (** XXX *)
-Definition interpret_binop {C: VyperConfig} (op: binop) (a b: uint256)
+Definition interpret_binop (op: binop) (a b: uint256)
 : expr_result uint256
 := ExprSuccess a.
 
-Record calldag {C: VyperConfig} := {
+Record calldag := {
   cd_declmap:  string -> option decl;
-  cd_depthmap: string -> option N;
+  cd_depthmap: string -> option nat;
   cd_depthmap_ok:
     forall name: string,
       match cd_declmap name with
@@ -50,14 +54,15 @@ Record calldag {C: VyperConfig} := {
               FSet.for_all (decl_callset decl)
                            (fun callee => match cd_depthmap callee with
                                           | None => false
-                                          | Some y => (y <? x)%N
+                                          | Some y => y <? x
                                           end)
                = true
             end
       end;
 }.
 
-Fixpoint bind_args {C: VyperConfig} (names: list string) (values: list uint256)
+(** Initialize a map of local variables with argument names and argument values. *)
+Fixpoint bind_args (names: list string) (values: list uint256)
 : string + string_map uint256
 := let _ := string_map_impl in
    match names with
@@ -79,8 +84,7 @@ Fixpoint bind_args {C: VyperConfig} (names: list string) (values: list uint256)
                  end
    end.
 
-Local Lemma interpret_call_helper {C: VyperConfig}
-                                  {this_decl: decl}
+Local Lemma interpret_call_helper {this_decl: decl}
                                   {fun_name: string}
                                   {arg_names: list string}
                                   {body: expr}
@@ -90,26 +94,24 @@ Proof.
 subst this_decl. unfold decl_callset. apply FSet.is_subset_refl.
 Qed.
 
-Lemma call_descend {C: VyperConfig}
-                   {call_depth_bound new_call_depth_bound current_fun_depth: nat}
+Lemma call_descend {call_depth_bound new_call_depth_bound current_fun_depth: nat}
                    (DepthOk : current_fun_depth < call_depth_bound)
                    (cd : calldag)
                    (this_fun_name: string)
                    (this_decl: decl)
                    (this_decl_ok: cd_declmap cd this_fun_name = Some this_decl)
                    (current_fun_depth_ok:
-                     cd_depthmap cd this_fun_name = Some (N.of_nat current_fun_depth))
+                     cd_depthmap cd this_fun_name = Some current_fun_depth)
                    (e : expr)
                    (CallOk : let _ := string_set_impl in
                              FSet.is_subset (expr_callset e) (decl_callset this_decl) = true)
                    (Ebound : call_depth_bound = S new_call_depth_bound)
                    (name : string)
                    (args : list expr)
-                   (E : e = PrivateOrBuiltinCall name args):
-  match cd_depthmap cd name with
-    | Some y => (y <? N.of_nat new_call_depth_bound)%N
-    | None => false
-    end = true.
+                   (E : e = PrivateOrBuiltinCall name args)
+                   {depth: nat}
+                   (Edepth: cd_depthmap cd name = Some depth):
+  depth < new_call_depth_bound.
 Proof.
 subst e. cbn in CallOk.
 assert(HasName: let _ := string_set_impl in FSet.has (decl_callset this_decl) name = true).
@@ -127,195 +129,238 @@ rewrite FSet.for_all_ok in K.
 assert (L := K name HasName). clear K.
 subst call_depth_bound.
 apply lt_n_Sm_le in DepthOk.
-destruct (cd_depthmap cd name). 2:{ assumption. }
-rewrite N.ltb_lt. rewrite N.ltb_lt in L.
-refine (N.lt_le_trans _ _ _ L _).
-rewrite<- N.compare_le_iff.
-rewrite<- Nat2N.inj_compare.
-rewrite Nat.compare_le_iff.
-exact DepthOk.
+rewrite Edepth in L.
+destruct current_fun_depth. { discriminate. }
+rewrite Nat.leb_le in L.
+rewrite Nat.le_succ_l in DepthOk.
+apply (Nat.le_lt_trans _ _ _ L DepthOk).
 Qed.
 
-Fixpoint interpret_call {C: VyperConfig}
-                        (CALL_depth_bound: nat)
-                        (call_depth_bound: nat)
-                        (current_fun_depth: nat)
-                        (DepthOk: current_fun_depth < call_depth_bound)
-                        (cd: calldag)
+Record fun_ctx (cd: calldag) (bound: nat) := {
+  fun_name: string;
+  fun_depth: nat;
+  fun_depth_ok: cd_depthmap cd fun_name = Some fun_depth;
+  fun_decl: decl;
+  fun_decl_ok: cd_declmap cd fun_name = Some fun_decl;
+  fun_bound_ok: fun_depth < bound;
+}.
+Arguments fun_name     {_ _}.
+Arguments fun_depth    {_ _}.
+Arguments fun_depth_ok {_ _}.
+Arguments fun_decl     {_ _}.
+Arguments fun_decl_ok  {_ _}.
+Arguments fun_bound_ok {_ _}.
+
+Local Lemma fun_ctx_descend_helper {cd: calldag}
+                                   {name: string}
+                                   {d: decl}
+                                   (Edecl : cd_declmap cd name = Some d):
+  cd_depthmap cd name <> None.
+Proof.
+assert (D := cd_depthmap_ok cd name).
+rewrite Edecl in D.
+intro H.
+rewrite H in D.
+exact D.
+Qed.
+
+(** Make a callee context from a caller context and a call expression, 
+  The None result means that no declaration with the given name is found.
+  No check is made that the callee context is indeed a function.
+  The max stack depth bound is reduced by 1.
+ *)
+Definition fun_ctx_descend {call_depth_bound new_call_depth_bound}
+                           {cd : calldag}
+                           {e : expr}
+                           {name : string}
+                           {args : list expr}
+
+                           (fc: fun_ctx cd call_depth_bound)
+                           (CallOk : let _ := string_set_impl in
+                                       FSet.is_subset (expr_callset e)
+                                                      (decl_callset (fun_decl fc))
+                                        = true)
+                           (Ebound : call_depth_bound = S new_call_depth_bound)
+                           (E: e = PrivateOrBuiltinCall name args)
+: option (fun_ctx cd new_call_depth_bound)
+:= match cd_declmap cd name as maybe_decl return _ = maybe_decl -> _ with
+   | None => fun _ =>
+       (* no declaration found - could be a builtin *)
+       None
+   | Some d => fun Edecl =>
+       match cd_depthmap cd name as maybe_depth return _ = maybe_depth -> _ with
+       | None => fun Edepth => False_rect _ (fun_ctx_descend_helper Edecl Edepth)
+       | Some depth => fun Edepth =>
+           Some {| fun_name := name
+                 ; fun_depth := depth
+                 ; fun_depth_ok := Edepth
+                 ; fun_decl := d
+                 ; fun_decl_ok := Edecl
+                 ; fun_bound_ok := call_descend (fun_bound_ok fc) cd (fun_name fc)
+                                                (fun_decl fc) (fun_decl_ok fc)
+                                                (fun_depth_ok fc) e CallOk Ebound 
+                                                name args E Edepth
+                |}
+       end eq_refl
+   end eq_refl.
+
+(*************************************************************************************************)
+
+Fixpoint interpret_call {call_depth_bound: nat}
+                        {cd: calldag}
+                        (fc: fun_ctx cd call_depth_bound)
                         (world: world_state)
-                        (fun_name: string)
                         (arg_values: list uint256)
+{struct call_depth_bound}
 : world_state * expr_result uint256
-:= match cd_declmap cd fun_name with
-   | Some this_decl =>
-      match this_decl as this_decl' return this_decl = this_decl' -> _ with
+:= let interpret_expr 
+   := fix interpret_expr
+         (world: world_state)
+         (loc: string_map uint256)
+         (e: expr)
+         (CallOk: let _ := string_set_impl in 
+                  FSet.is_subset (expr_callset e) (decl_callset (fun_decl fc)) = true)
+      {struct e}
+      : world_state * expr_result uint256
+      := let interpret_expr_list
+         := fix interpret_expr_list (world: world_state)
+                                    (loc: string_map uint256)
+                                    (e: list expr)
+                                    (CallOk: let _ := string_set_impl in 
+                                             FSet.is_subset (expr_list_callset e)
+                                                            (decl_callset (fun_decl fc))
+                                             = true)
+            {struct e}
+            : world_state * expr_result (list uint256)
+            := match e as e' return e = e' -> _ with
+               | nil => fun _ => (world, ExprSuccess nil)
+               | (h :: t)%list => fun E =>
+                   let (world', result_h) := interpret_expr world loc h
+                                                            (callset_descend_head E CallOk)
+                   in match result_h with
+                      | ExprError msg => (world', ExprError msg)
+                      | ExprSuccess x =>
+                         let (world'', result_t) := interpret_expr_list world' loc t
+                                                                        (callset_descend_tail E CallOk)
+                         in (world'', match result_t with
+                                      | ExprError _ => result_t
+                                      | ExprSuccess y => ExprSuccess (x :: y)%list
+                                      end)
+                       end
+               end eq_refl
+         in match call_depth_bound as call_depth_bound' return _ = call_depth_bound' -> _ with
+            | O => fun Ebound => False_rect _ (Nat.nlt_0_r (fun_depth fc)
+                                                           (eq_ind _ _ (fun_bound_ok fc) _ Ebound))
+            | S new_call_depth_bound => fun Ebound =>
+
+                 match e as e' return e = e' -> _ with
+                 | Const val => fun _ => (world, ExprSuccess val)
+                 | LocalVar name => fun _ =>
+                     let _ := string_map_impl in
+                     (world, match Map.lookup loc name with
+                             | Some val => ExprSuccess val
+                             | None => ExprError "Local variable not found"
+                             end)
+                 | StorageVar name => fun _ => 
+                     let _ := string_map_impl in
+                     (world, match storage_lookup world name with
+                             | Some val => ExprSuccess val
+                             | None => ExprError "Storage variable not found"
+                             end)
+                 | UnOp op a => fun E =>
+                     let (world', result) := interpret_expr world loc a
+                                                            (callset_descend_unop E CallOk)
+                     in (world', match result with
+                                 | ExprSuccess val => interpret_unop op val
+                                 | ExprError msg => result
+                                 end)
+                 | BinOp op a b => fun E =>
+                     let (world', result_a) := interpret_expr world loc a
+                                                              (callset_descend_binop_left E CallOk)
+                     in match result_a with
+                     | ExprError msg => (world', result_a)
+                     | ExprSuccess x =>
+                       let (world'', result_b) := interpret_expr world' loc b
+                                                                 (callset_descend_binop_right E CallOk)
+                       in (world'', match result_b with
+                                    | ExprError msg => result_b
+                                    | ExprSuccess y => interpret_binop op x y
+                                    end)
+                     end
+                 (* | IfThenElse cond yes no => fun E =>
+                     _ *)
+                 | PrivateOrBuiltinCall name args => fun E =>
+                     let (world', result_args) :=
+                       interpret_expr_list world loc args
+                                           (callset_descend_args E CallOk)
+                     in match result_args with
+                        | ExprError msg => (world', ExprError msg)
+                        | ExprSuccess arg_values =>
+                            match fun_ctx_descend fc CallOk Ebound E with
+                            | None => (* can't resolve the function, maybe it's a builtin *)
+                                      (world', ExprError "can't resolve function name")
+                            | Some new_fc => interpret_call new_fc world' arg_values
+                            end
+                        end
+                 end eq_refl
+         end eq_refl
+   in match fun_decl fc as d return _ = d -> _ with
       | FunDecl _ arg_names body => fun E =>
           match bind_args arg_names arg_values with
           | inl err => (world, ExprError err)
-          | inr loc => interpret_expr CALL_depth_bound call_depth_bound
-                                      current_fun_depth DepthOk
-                                      cd this_decl
-                                      world loc body
-                                      (interpret_call_helper E)
+          | inr loc => interpret_expr world loc body (interpret_call_helper E)
           end
-     | _ => fun _ => (world, ExprError "a declaration is found but it's not a function")
-     end eq_refl
-   | None => (world, ExprError "declaration not found") (* XXX: builtins *)
-   end
-with interpret_expr {C: VyperConfig}
-                    (CALL_depth_bound: nat)
-                    (call_depth_bound: nat)
-                    (current_fun_depth: nat)
-                    (DepthOk: current_fun_depth < call_depth_bound)
-                    (cd: calldag)
-                    (this_decl: decl)
-                    (world: world_state)
-                    (loc: string_map uint256)
-                    (e: expr)
-                    (CallOk: let _ := string_set_impl in 
-                             FSet.is_subset (expr_callset e) (decl_callset this_decl) = true)
-: world_state * expr_result uint256
-:= let interpret_expr_list := 
-     fix interpret_expr_list {C: VyperConfig}
-                             (CALL_depth_bound: nat)
-                             (call_depth_bound: nat)
-                             (current_fun_depth: nat)
-                             (DepthOk: current_fun_depth < call_depth_bound)
-                             (cd: calldag)
-                             (this_decl: decl)
-                             (world: world_state)
-                             (loc: string_map uint256)
-                             (e: list expr)
-                             (CallOk: let _ := string_set_impl in 
-                                      FSet.is_subset (expr_list_callset e) (decl_callset this_decl) = true)
-     {struct e}
-     : world_state * expr_result (list uint256)
-     := match e as e' return e = e' -> _ with
-        | nil => fun _ => (world, ExprSuccess nil)
-        | (h :: t)%list => fun E =>
-            let (world', result_h) := interpret_expr CALL_depth_bound call_depth_bound
-                                                     current_fun_depth DepthOk
-                                                     cd this_decl
-                                                     world loc h
-                                                     (callset_descend_head E CallOk)
-            in match result_h with
-               | ExprError msg => (world', ExprError msg)
-               | ExprSuccess x =>
-                  let (world'', result_t) := interpret_expr_list CALL_depth_bound call_depth_bound
-                                                                 current_fun_depth DepthOk
-                                                                 cd this_decl
-                                                                 world' loc t
-                                                                 (callset_descend_tail E CallOk)
-                  in (world'', match result_t with
-                               | ExprError _ => result_t
-                               | ExprSuccess y => ExprSuccess (x :: y)%list
-                               end)
-                end
-        end eq_refl
-   in match CALL_depth_bound as CALL_depth_bound' return CALL_depth_bound = CALL_depth_bound' -> _
-   with
-   | O => fun _ => (world, ExprError "Max CALL stack depth exceeded")
-   | S new_CALL_depth_bound => fun _ =>
-        match call_depth_bound as call_depth_bound'
-          return call_depth_bound = call_depth_bound' -> _
-        with
-        | O => fun E => False_rect _ (Nat.nlt_0_r current_fun_depth
-                                                  (eq_ind _ _ DepthOk _ E))
-        | S new_call_depth_bound => fun _ =>
+      | _ => fun _ => (world, ExprError "a declaration is found but it's not a function")
+      end eq_refl.
 
-            match e as e' return e = e' -> _ with
-               | Const val => fun _ => (world, ExprSuccess val)
-               | LocalVar name => fun _ =>
-                   let _ := string_map_impl in
-                   (world, match Map.lookup loc name with
-                           | Some val => ExprSuccess val
-                           | None => ExprError "Local variable not found"
-                           end)
-               | StorageVar name => fun _ => 
-                   let _ := string_map_impl in
-                   (world, match storage_lookup world name with
-                           | Some val => ExprSuccess val
-                           | None => ExprError "Storage variable not found"
-                           end)
-               | UnOp op a => fun E =>
-                   let (world', result) := interpret_expr CALL_depth_bound call_depth_bound
-                                                          current_fun_depth DepthOk cd
-                                                          this_decl world loc a
-                                                          (callset_descend_unop E CallOk)
-                   in (world', match result with
-                               | ExprSuccess val => interpret_unop op val
-                               | ExprError msg => result
-                               end)
-               | BinOp op a b => fun E =>
-                   let (world', result_a) := interpret_expr CALL_depth_bound call_depth_bound
-                                                            current_fun_depth DepthOk cd
-                                                            this_decl world loc a
-                                                            (callset_descend_binop_left E CallOk)
-                   in match result_a with
-                   | ExprError msg => (world', result_a)
-                   | ExprSuccess x =>
-                     let (world'', result_b) := interpret_expr CALL_depth_bound call_depth_bound
-                                                               current_fun_depth DepthOk cd
-                                                               this_decl world' loc b
-                                                               (callset_descend_binop_right E CallOk)
-                     in (world'', match result_b with
-                                  | ExprError msg => result_b
-                                  | ExprSuccess y => interpret_binop op x y
-                                  end)
-                   end
-               (* | IfThenElse cond yes no => fun E =>
-                   _ *)
-               | PrivateOrBuiltinCall name args => fun E =>
-                   let (world', result_args) :=
-                     interpret_expr_list CALL_depth_bound call_depth_bound
-                                         current_fun_depth DepthOk cd
-                                         this_decl world loc args
-                                         (callset_descend_args E CallOk)
-                   in match result_args with
-                      | ExprError msg => (world', ExprError msg)
-                      | ExprSuccess arg_values =>
-                          _
-(*
-                          interpret_call CALL_depth_bound new_call_depth_bound
-                                         XXX
-                        (current_fun_depth: nat)
-                        (DepthOk: current_fun_depth < call_depth_bound)
-                        (cd: calldag)
-                        (world: world_state)
-                        (fun_name: string)
-                        (arg_values: list uint256) *)
-                      end
-               end eq_refl
-        end eq_refl
+Local Lemma make_fun_ctx_helper {cd: calldag}
+                          {name: string}
+                          {d : decl}
+                          (Ed : cd_declmap cd name = Some d)
+                          (Edepth : cd_depthmap cd name = None):
+  False.
+Proof.
+assert (W := cd_depthmap_ok cd name).
+rewrite Ed in W. rewrite Edepth in W. exact W.
+Qed.
+
+Definition make_fun_ctx_and_bound (cd: calldag)
+                                  (name: string)
+: option { bound: nat & fun_ctx cd bound }
+:= match cd_declmap cd name as maybe_d return _ = maybe_d -> _ with
+   | None => fun _ => None
+   | Some d => fun Ed =>
+      match cd_depthmap cd name as depth' return _ = depth' -> _ with
+      | None => fun Edepth => False_rect _ (make_fun_ctx_helper Ed Edepth)
+      | Some depth => fun Edepth => Some (existT _
+                                                 (S depth)
+                                                 {| fun_name := name
+                                                  ; fun_decl := d
+                                                  ; fun_decl_ok := Ed
+                                                  ; fun_depth := depth
+                                                  ; fun_depth_ok := Edepth
+                                                  ; fun_bound_ok := Nat.lt_succ_diag_r _
+                                                 |})
+      end eq_refl
    end eq_refl.
 
+(** This is a simplified interface to interpret_call that takes care of creating a function context. *)
+Definition interpret (cd: calldag)
+                     (function_name: string)
+                     (world: world_state)
+                     (arg_values: list uint256)
+: world_state * expr_result uint256
+:= match make_fun_ctx_and_bound cd function_name with
+   | None => (world, ExprError "declaration not found")
+   | Some (existT _ bound fc) => interpret_call fc world arg_values
+   end.
 
-Definition interpret_expr {C: VyperConfig}
-                          (CALL_depth_bound: nat)
-                          (call_depth_bound: nat)
-                          (current_fun_depth: nat)
-                          (DepthOk: current_fun_depth < call_depth_bound)
-                          (cd: calldag)
-                          (allowed_calls: string_set)
-                          (world: world_state)
-                          (loc: string_map uint256)
-                          (e: expr)
-                          (CallOk: let _ := string_set_impl in 
-                                   FSet.is_subset (expr_callset e) allowed_calls = true)
-: world_state * expr_result uint256. admit. Admitted.
-
+(*
 Definition stmt_is_local_var_decl {C: VyperConfig} (s: stmt)
 := match s with
    | LocalVarDecl _ _ => true
    | _ => false
    end.
-
-Fixpoint interpret_call {C: VyperConfig}
-                        (call_depth_bound: nat)
-                        (cd: calldag)
-                        (fun_name: string)
-                        (allowed_calls: string_set)
-                        (world: world_state)
 
 
 Fixpoint interpret_stmt {C: VyperConfig}
@@ -370,5 +415,6 @@ Fixpoint interpret_stmt_list {C: VyperConfig}
    | FixedRangeLoop (var: string) (start: option uint256) (stop: uint256) (body: list stmt)
    | FixedCountLoop (var: string) (start: string) (count: uint256) (body: list stmt).
    end.
+*)
 
-Definition interpret 
+End Interpret.
