Graph/MaxLenPath.v
@@ -1,0 +1,216 @@
+From Coq Require Import NArith List.
+From Coq Require Import FMapPositive.
+
+Require Path.
+
+
+(* A path that has maximal length among those starting at the same vertex. *)
+Record max_len_path {V: Type} (R: V -> V -> Prop)
+:= {
+    mlp_start: V;
+    mlp_path: Path.t R mlp_start;
+    mlp_len: N;
+    mlp_len_ok: mlp_len = N.of_nat (Path.length mlp_path);
+    mlp_ok: forall q: Path.t R mlp_start,
+              Path.length q <= Path.length mlp_path
+   }.
+Arguments mlp_start  {_ _}.
+Arguments mlp_path   {_ _}.
+Arguments mlp_len    {_ _}.
+Arguments mlp_len_ok {_ _}.
+Arguments mlp_ok     {_ _}.
+
+(* A maximal length path among those that start with vertices in the specified list. *)
+Record max_len_path_nonempty_list {V: Type} (R: V -> V -> Prop)
+                                  (vs: list V)
+:= {
+    mlpn_start: V;
+    mlpn_path: Path.t R mlpn_start;
+    mlpn_In: In mlpn_start vs;
+    mlpn_len: N;
+    mlpn_len_ok: mlpn_len = N.of_nat (Path.length mlpn_path);
+    mlpn_ok: forall (v: V)
+                     (q: Path.t R v),
+                In v vs -> Path.length q <= Path.length mlpn_path;
+   }.
+Arguments mlpn_start  {_ _ _}.
+Arguments mlpn_path   {_ _ _}.
+Arguments mlpn_In     {_ _ _}.
+Arguments mlpn_len    {_ _ _}.
+Arguments mlpn_len_ok {_ _ _}.
+Arguments mlpn_ok     {_ _ _}.
+
+(* A helper for max_len_path_cons_nonempty. *)
+Lemma max_len_path_cons_tail {V: Type} {R: V -> V -> Prop} {vs: list V}
+                             (h: max_len_path R)
+                             (t: max_len_path_nonempty_list R vs)
+                             (E: (mlp_len h <=? mlpn_len t)%N = true)
+                             (v: V)
+                             (q: Path.t R v)
+                             (H: In v (mlp_start h :: vs)):
+    Path.length q <= Path.length (mlpn_path t).
+Proof.
+cbn in H.
+destruct H. 2: exact (mlpn_ok t v q H).
+subst.
+assert (L := mlp_ok h q).
+apply N.leb_le in E.
+rewrite mlp_len_ok in E. rewrite mlpn_len_ok in E.
+rewrite<- N.compare_le_iff in E.
+rewrite<- Nat2N.inj_compare in E.
+rewrite PeanoNat.Nat.compare_le_iff in E.
+exact (PeanoNat.Nat.le_trans _ _ _ L E).
+Qed.
+
+(* A helper for max_len_path_cons_nonempty. *)
+Lemma max_len_path_cons_head {V: Type} {R: V -> V -> Prop} {vs: list V}
+                             (h: max_len_path R)
+                             (t: max_len_path_nonempty_list R vs)
+                             (E: (mlp_len h <=? mlpn_len t)%N = false)
+                             (v: V)
+                             (q: Path.t R v)
+                             (H: In v (mlp_start h :: vs)):
+    Path.length q <= Path.length (mlp_path h).
+Proof.
+cbn in H.
+destruct H. { subst. exact (mlp_ok h q). }
+assert(T := mlpn_ok t v q H).
+apply N.leb_gt in E.
+rewrite mlp_len_ok in E. rewrite mlpn_len_ok in E.
+rewrite<- N.compare_lt_iff in E.
+rewrite<- Nat2N.inj_compare in E.
+rewrite PeanoNat.Nat.compare_lt_iff in E.
+apply PeanoNat.Nat.lt_le_incl.
+exact (PeanoNat.Nat.le_lt_trans _ _ _ T E).
+Qed.
+
+(* This is how to grow the list of max_len_path_nonempty_list. *)
+Definition max_len_path_cons_nonempty {V: Type} {R: V -> V -> Prop}
+                                      {vs: list V}
+                                      (h: max_len_path R)
+                                      (t: max_len_path_nonempty_list R vs)
+  : max_len_path_nonempty_list R (mlp_start h :: vs)
+  := let f := N.leb (mlp_len h) (mlpn_len t) in
+     match f as f' return (f = f' -> _) with
+     | true => fun E => {|
+                           mlpn_start := mlpn_start t;
+                           mlpn_path := mlpn_path t;
+                           mlpn_In := in_cons _ _ _ (mlpn_In t);
+                           mlpn_len := mlpn_len t;
+                           mlpn_len_ok := mlpn_len_ok t;
+                           mlpn_ok := max_len_path_cons_tail h t E;
+                         |}
+     | false => fun E => {|
+                           mlpn_start := mlp_start h;
+                           mlpn_path := mlp_path h;
+                           mlpn_In := in_eq _ _;
+                           mlpn_len := mlp_len h;
+                           mlpn_len_ok := mlp_len_ok h;
+                           mlpn_ok := max_len_path_cons_head h t E;
+                          |}
+     end eq_refl.
+
+(* Since we can't start growing the list of max_len_path_nonempty_list
+   from an empty list, we have to start from singletons.
+   We can convert max_len_path to max_len_path_nonempty_list of a singleton.
+ *)
+Program Definition max_len_path_single {V: Type} {R: V -> V -> Prop}
+                                       (m: max_len_path R)
+: max_len_path_nonempty_list R (mlp_start m :: nil)
+:= {|
+    mlpn_start := mlp_start m;
+    mlpn_path := mlp_path m;
+    mlpn_In := in_eq _ _;
+    mlpn_len := mlp_len m;
+    mlpn_len_ok := mlp_len_ok m;
+    mlpn_ok := _;
+  |}.
+Next Obligation.
+destruct H; [|contradiction]. subst.
+exact (mlp_ok m q).
+Qed.
+
+(* A wrapper for max_len_path_nonempty_list that takes the empty list as a special case. *)
+Inductive max_len_path_for_list {V: Type} (R: V -> V -> Prop)
+                                (vs: list V)
+:= MLPL_Empty (Ok: vs = nil)
+ | MLPL_Nonempty (m: max_len_path_nonempty_list R vs).
+Arguments MLPL_Empty    {_ _ _}.
+Arguments MLPL_Nonempty {_ _ _}.
+
+(* Finally a nice-looking cons for max_len_path_for_list. *)
+Program Definition max_len_path_cons {V: Type} {R: V -> V -> Prop}
+                                     {vs: list V}
+                                     (h: max_len_path R)
+                                     (t: max_len_path_for_list R vs)
+  : max_len_path_for_list R (mlp_start h :: vs)
+  := MLPL_Nonempty (match t with
+                    | MLPL_Empty is_nil => max_len_path_single h
+                    | MLPL_Nonempty m => max_len_path_cons_nonempty h m
+                    end).
+
+Program Definition max_len_path_collect_nonempty
+                                {V: Type} {R: V -> V -> Prop}
+                                {vs: list V}
+                                (m: max_len_path_nonempty_list R vs)
+                                (u: V)
+                                (Ok: forall v, In v vs <-> R u v)
+  : max_len_path R
+  := {|
+      mlp_start := u;
+      mlp_path := Path.Cons _ (proj1 (Ok _) (mlpn_In m)) (mlpn_path m);
+      mlp_len := N.succ (mlpn_len m);
+      mlp_len_ok := _;
+      mlp_ok := _;
+    |}.
+Next Obligation.
+  rewrite (mlpn_len_ok m).
+  now rewrite<- Nat2N.inj_succ.
+Qed.
+Next Obligation.
+  destruct q; cbn. { auto with arith. }
+  apply le_n_S.
+  apply (mlpn_ok m v q).
+  now rewrite Ok.
+Qed.
+
+Program Definition max_len_path_collect_empty {V: Type} {R: V -> V -> Prop}
+                                              {vs: list V}
+                                              (E: vs = nil)
+                                              (u: V)
+                                              (Ok: forall v, In v vs <-> R u v)
+: max_len_path R
+:= {|
+    mlp_start := u;
+    mlp_path := Path.Nil u;
+    mlp_len := N0;
+    mlp_len_ok := eq_refl;
+    mlp_ok := _;
+  |}.
+Next Obligation.
+destruct q. { auto. }
+exfalso.
+now rewrite<- Ok in *.
+Qed.
+
+(* collect builds a max_len_path for a vertex from max_len_path_for_list for the fanout set. *)
+Definition max_len_path_collect {V: Type} {R: V -> V -> Prop}
+                                {vs: list V}
+                                (m: max_len_path_for_list R vs)
+                                (u: V)
+                                (Ok: forall v, In v vs <-> R u v)
+  : max_len_path R
+  := match m with
+     | MLPL_Empty is_nil => max_len_path_collect_empty is_nil u Ok
+     | MLPL_Nonempty m => max_len_path_collect_nonempty m u Ok
+     end.
+
+Lemma max_len_path_collect_start {V: Type} {R: V -> V -> Prop}
+                                 {vs: list V}
+                                 (m: max_len_path_for_list R vs)
+                                 (u: V)
+                                 (Ok: forall v, In v vs <-> R u v):
+  mlp_start (max_len_path_collect m u Ok) = u.
+Proof.
+  now destruct m.
+Qed.
